module solver2 (ğ”¸ : Set) where

open import Relation.Binary.PropositionalEquality

module _ {A : Set} where
  open import Algebra.Definitions {A = A} _â‰¡_ public

postulate
  0# 1# : ğ”¸
  _+_ _*_ : ğ”¸ â†’ ğ”¸ â†’ ğ”¸
  +-identityË¡ : LeftIdentity 0# _+_
  +-identityÊ³ : RightIdentity 0# _+_
  *-identityË¡ : LeftIdentity 1# _*_
  *-identityÊ³ : RightIdentity 1# _*_
  *-zeroË¡ : LeftZero 0# _*_
  *-zeroÊ³ : RightZero 0# _*_
  +-comm : Commutative _+_
  *-comm : Commutative _*_
  +-assoc : Associative _+_
  *-assoc : Associative _*_
  *-distribË¡-+ : _*_ DistributesOverË¡ _+_
  *-distribÊ³-+ : _*_ DistributesOverÊ³ _+_

infixr 5 _+_
infixr 6 _*_

open import Data.Nat
  using (â„•; zero; suc)

private variable
  n : â„•

data HNF : â„• â†’ Set where
  const : ğ”¸ â†’ HNF zero
  coeff : HNF n â†’ HNF (suc n)
  _*x+_ : HNF (suc n) â†’ HNF n â†’ HNF (suc n)

_+H_ : HNF n â†’ HNF n â†’ HNF n
const x +H const xâ‚ = const (x + xâ‚)
coeff x +H coeff xâ‚ = coeff (x +H xâ‚)
coeff x +H (xâ‚ *x+ xâ‚‚) = xâ‚ *x+ (x +H xâ‚‚)
(x *x+ xâ‚) +H coeff xâ‚‚ = x *x+ (xâ‚ +H xâ‚‚)
(x *x+ xâ‚) +H (xâ‚‚ *x+ xâ‚ƒ) = (x +H xâ‚‚) *x+ (xâ‚ +H xâ‚ƒ)
infixr 5 _+H_

â†ª : ğ”¸ â†’ HNF n
â†ª {zero} x = const x
â†ª {suc n} x = coeff (â†ª x)

0H : HNF n
0H = â†ª 0#

1H : HNF n
1H = â†ª 1#

x* : HNF (suc n) â†’ HNF (suc n)
x* x = x *x+ 0H

_*H_ : HNF n â†’ HNF n â†’ HNF n
const x *H const xâ‚ = const (x * xâ‚)
coeff x *H coeff xâ‚ = coeff (x *H xâ‚)
coeff x *H (xâ‚ *x+ xâ‚‚) = (coeff x *H xâ‚) *x+ (x *H xâ‚‚)
(x *x+ xâ‚) *H coeff xâ‚‚ = (x *H coeff xâ‚‚) *x+ (xâ‚ *H xâ‚‚)
(x *x+ xâ‚) *H (xâ‚‚ *x+ xâ‚ƒ) = x* (x* (x *H xâ‚‚)) +H x* ((x *H coeff xâ‚ƒ) +H (xâ‚‚ *H coeff xâ‚)) +H coeff (xâ‚ *H xâ‚ƒ)
infixr 6 _*H_


open import Data.Fin
  using (Fin; suc; zero)

data Syn (n : â„•) : Set where
  var : Fin n â†’ Syn n
  con : ğ”¸ â†’ Syn n
  _:+_ : Syn n â†’ Syn n â†’ Syn n
  _:*_ : Syn n â†’ Syn n â†’ Syn n

âŸ¦_âŸ§ : Syn n â†’ (Fin n â†’ ğ”¸) â†’ ğ”¸
âŸ¦ var v âŸ§  vs = vs v
âŸ¦ con c âŸ§  vs = c
âŸ¦ x :+ y âŸ§ vs = âŸ¦ x âŸ§ vs + âŸ¦ y âŸ§ vs
âŸ¦ x :* y âŸ§ vs = âŸ¦ x âŸ§ vs * âŸ¦ y âŸ§ vs

open import Function using (_âˆ˜_)

to-var : Fin n â†’ HNF n
to-var zero = x* 1H
to-var (suc x) = coeff (to-var x)

normalize : Syn n â†’ HNF n
normalize (var x) = to-var x
normalize (con x) = â†ª x
normalize (x :+ xâ‚) = normalize x +H normalize xâ‚
normalize (x :* xâ‚) = normalize x *H normalize xâ‚

eval : (Fin n â†’ ğ”¸) â†’ HNF n â†’ ğ”¸
eval v (const x) = x
eval v (coeff x) = eval (v âˆ˜ suc) x
eval v (x *x+ xâ‚) = v zero * eval v x + eval (v âˆ˜ suc) xâ‚

eval-â†ª : (f : Fin n â†’ ğ”¸) â†’ (x : ğ”¸) â†’ eval f (â†ª x) â‰¡ x
eval-â†ª {zero} f x = refl
eval-â†ª {suc n} f x = eval-â†ª (f âˆ˜ suc) x

eval-to-var : (f : Fin n â†’ ğ”¸) â†’ (x : Fin n) â†’ eval f (to-var x) â‰¡ f x
eval-to-var f zero
  rewrite eval-â†ª (f âˆ˜ suc) 0#
  rewrite eval-â†ª (f âˆ˜ suc) 1#
  rewrite *-identityÊ³ (f zero)
    = +-identityÊ³ (f zero)
eval-to-var f (suc x) = eval-to-var (f âˆ˜ suc) x

postulate
  â€¦algebraâ€¦ : {x y : ğ”¸} â†’ x â‰¡ y
  â€¦viaâ€¦ : {B : Set} {x y : ğ”¸} â†’ B â†’ x â‰¡ y

+-hom : (f : Fin n â†’ ğ”¸) â†’ (hâ‚ hâ‚‚ : HNF n) â†’ eval f (hâ‚ +H hâ‚‚) â‰¡ eval f hâ‚ + eval f hâ‚‚
+-hom f (const x) (const xâ‚) = refl
+-hom f (coeff hâ‚) (coeff hâ‚‚) = +-hom (f âˆ˜ suc) hâ‚ hâ‚‚
+-hom f (coeff hâ‚) (hâ‚‚ *x+ hâ‚ƒ)
  rewrite +-hom (f âˆ˜ suc) hâ‚ hâ‚ƒ
    = begin
      f zero * eval f hâ‚‚ + eval f' hâ‚ + eval f' hâ‚ƒ
    â‰¡âŸ¨ â€¦algebraâ€¦ âŸ©
      eval f' hâ‚ + f zero * eval f hâ‚‚ + eval f' hâ‚ƒ
    âˆ
  where
    f' = f âˆ˜ suc
    open â‰¡-Reasoning
+-hom f (hâ‚ *x+ hâ‚‚) (coeff hâ‚ƒ)
  rewrite +-hom (f âˆ˜ suc) hâ‚‚ hâ‚ƒ = sym (+-assoc _ _ _)
+-hom f (hâ‚ *x+ hâ‚‚) (hâ‚ƒ *x+ hâ‚„)
  rewrite +-hom f hâ‚ hâ‚ƒ
  rewrite +-hom (f âˆ˜ suc) hâ‚‚ hâ‚„ = begin
      f zero * (eval f hâ‚ + eval f hâ‚ƒ)
        + (eval f' hâ‚‚ + eval f' hâ‚„)
    â‰¡âŸ¨ â€¦algebraâ€¦ âŸ©
      (f zero * eval f hâ‚ + eval f' hâ‚‚)
        + f zero * eval f hâ‚ƒ + eval f' hâ‚„
    âˆ
  where
    f' = f âˆ˜ suc
    open â‰¡-Reasoning

*-hom : (f : Fin n â†’ ğ”¸) â†’ (hâ‚ hâ‚‚ : HNF n) â†’ eval f (hâ‚ *H hâ‚‚) â‰¡ eval f hâ‚ * eval f hâ‚‚
*-hom f (const x) (const xâ‚) = refl
*-hom f (coeff hâ‚) (coeff hâ‚‚) = *-hom (f âˆ˜ suc) hâ‚ hâ‚‚
*-hom f (coeff hâ‚) (hâ‚‚ *x+ hâ‚ƒ)
  rewrite *-hom f (coeff hâ‚) hâ‚‚
  rewrite *-hom (f âˆ˜ suc) hâ‚ hâ‚ƒ =
    begin
      f zero * eval f' hâ‚ * eval f hâ‚‚ + eval f' hâ‚ * eval f' hâ‚ƒ
    â‰¡âŸ¨ â€¦algebraâ€¦ âŸ©
      eval f' hâ‚ * f zero * eval f hâ‚‚ + eval f' hâ‚ * eval f' hâ‚ƒ
    â‰¡âŸ¨ sym (*-distribË¡-+ _ _ _) âŸ©
      eval f' hâ‚ * (f zero * eval f hâ‚‚ + eval f' hâ‚ƒ)
    âˆ
  where
    f' = f âˆ˜ suc
    open â‰¡-Reasoning
*-hom f (hâ‚ *x+ hâ‚‚) (coeff hâ‚ƒ)
  rewrite *-hom (f âˆ˜ suc) hâ‚‚ hâ‚ƒ
  rewrite *-hom f hâ‚ (coeff hâ‚ƒ) =
    begin
      f zero * eval f hâ‚ * eval f' hâ‚ƒ + eval f' hâ‚‚ * eval f' hâ‚ƒ
    â‰¡âŸ¨ â€¦algebraâ€¦ âŸ©
      (f zero * eval f hâ‚) * eval f' hâ‚ƒ + eval f' hâ‚‚ * eval f' hâ‚ƒ
    â‰¡âŸ¨ sym (*-distribÊ³-+ _ _ _) âŸ©
      (f zero * eval f hâ‚ + eval f' hâ‚‚) * eval f' hâ‚ƒ
    âˆ
  where
    f' = f âˆ˜ suc
    open â‰¡-Reasoning
-- TODO(sandy):
*-hom f (hâ‚ *x+ hâ‚‚) (hâ‚ƒ *x+ hâ‚„) = â€¦algebraâ€¦


eval-norm : (f : Fin (n) â†’ ğ”¸) â†’ (s : Syn n) â†’ eval f (normalize s) â‰¡ âŸ¦ s âŸ§ f
eval-norm f (var x) = eval-to-var f x
eval-norm f (con x) = eval-â†ª f x
eval-norm f (s :+ sâ‚)
  rewrite +-hom f (normalize s) (normalize sâ‚)
  rewrite eval-norm f s
  rewrite eval-norm f sâ‚ = refl
eval-norm f (s :* sâ‚)
  rewrite *-hom f (normalize s) (normalize sâ‚)
  rewrite eval-norm f s
  rewrite eval-norm f sâ‚ = refl


open import Data.Vec using (Vec; []; _âˆ·_; map; lookup)

fins : Vec (Fin n) n
fins {zero} = []
fins {suc n} = zero âˆ· map suc fins

vars : Vec (Syn n) n
vars = map var fins

solve
    : (n : â„•)
    â†’ (x y : Vec (Syn n) n â†’ Syn n)
    â†’ (v : Vec ğ”¸ n)
    â†’ normalize (x vars) â‰¡ normalize (y vars)
    â†’ âŸ¦ x vars âŸ§ (lookup v) â‰¡ âŸ¦ y vars âŸ§ (lookup v)
solve n x y v x=y = begin
  âŸ¦ x vars âŸ§ f                 â‰¡âŸ¨ sym (eval-norm f (x vars)) âŸ©
  eval f (normalize (x vars))  â‰¡âŸ¨ cong (eval f) x=y âŸ©
  eval f (normalize (y vars))  â‰¡âŸ¨ eval-norm f (y vars) âŸ©
  âŸ¦ y vars âŸ§ f                 âˆ
  where
    f = lookup v
    open â‰¡-Reasoning

